awwwwww snap -- got something to verify

code/hash/Hacl.Hash.Lib.LoadStore.fst
@@ -175,6 +175,57 @@ let uint64s_from_be_bytes output input len =
 
 #reset-options " --max_fuel 0 --z3rlimit 100"
 
+
+val uint64s_from_le_bytes:
+  output:buffer H64.t ->
+  input:uint8_p{disjoint output input} ->
+  len:U32.t{length output = U32.v len /\ 8 * U32.v len = length input} ->
+  Stack unit
+    (requires (fun h -> live h output /\ live h input))
+    (ensures  (fun h0 _ h1 -> live h1 output /\ live h0 input /\ modifies_1 output h0 h1 /\
+      (let o = reveal_h64s (as_seq h1 output) in
+       let i = reveal_sbytes (as_seq h0 input) in
+       o == Spec.Lib.uint64s_from_le (U32.v len) i)))
+let uint64s_from_le_bytes output input len =
+  let h0 = ST.get() in
+  let inv (h1: mem) (i: nat): Type0 =
+    live h1 output /\ modifies_1 output h0 h1 /\ 0 <= i /\ i <= UInt32.v len
+    /\ Seq.slice (reveal_h64s (as_seq h1 output)) 0 i == Spec.Lib.uint64s_from_le i (reveal_sbytes (Seq.slice (as_seq h0 input) 0 (8 * i)))
+  in
+  let f' (i:UInt32.t{ FStar.UInt32.( 0 <= v i /\ v i < v len ) }): Stack unit
+    (requires (fun h -> inv h (UInt32.v i)))
+    (ensures (fun h_1 _ h_2 -> FStar.UInt32.(inv h_2 (v i + 1))))
+  = let h = ST.get() in
+    let open FStar.UInt32 in
+    assert(as_seq h input == as_seq h0 input);
+    let inputi = hload64_le (Buffer.sub input (8ul*^i) (8ul)) in
+    output.(i) <- inputi;
+    let h' = ST.get() in
+    Spec.Lib.lemma_uint64s_from_le_def_1 (UInt32.v i + 1) (reveal_sbytes (Seq.slice (as_seq h0 input) 0 (8 * v i + 8)));
+    Seq.lemma_eq_intro (Seq.slice (as_seq h0 input) 0 (8 * v i + 8))
+                       (Seq.append (Seq.slice (as_seq h0 input) 0 (8 * v i)) (as_seq h (Buffer.sub input (8ul *^ i) (8ul))));
+    Seq.lemma_eq_intro (as_seq h0 (Buffer.sub input (8ul*^i) (8ul)))
+                       (Seq.slice (as_seq h0 input) (8 * v i) (8 * v i + 8));
+    Seq.lemma_eq_intro (Seq.slice (as_seq h0 input) (8 * v i) (8 * v i + 8))
+                       (Seq.slice (Seq.slice (as_seq h0 input) 0 (8 * v i + 8)) (8 * v i) (8 * v i + 8));
+    Seq.lemma_eq_intro (Seq.slice (as_seq h0 input) 0 (8 * v i))
+                       (Seq.slice (Seq.slice (as_seq h0 input) 0 (8 * v i + 8)) 0 (8 * v i));
+    Seq.lemma_eq_intro (Seq.slice (as_seq h' output) 0 (v i+1))
+                       (Seq.snoc (Seq.slice (as_seq h output) 0 (v i)) inputi);
+    Seq.lemma_eq_intro (reveal_h64s (Seq.slice (as_seq h' output) 0 (v i + 1)))
+                       (Spec.Lib.uint64s_from_le (v i + 1) (reveal_sbytes (Seq.slice (as_seq h0 input) 0 (8 * (v i + 1)))))
+  in
+  Spec.Lib.lemma_uint64s_from_le_def_0 0 (reveal_sbytes (Seq.slice (as_seq h0 input) 0 0));
+  Seq.lemma_eq_intro (Seq.slice (as_seq h0 output) 0 0) Seq.createEmpty;
+  C.Loops.for 0ul len inv f';
+  let h = ST.get() in
+  Seq.lemma_eq_intro (Seq.slice (as_seq h output) 0 (UInt32.v len)) (as_seq h output);
+  Seq.lemma_eq_intro (Seq.slice (as_seq h0 input) 0 (8 * UInt32.v len)) (as_seq h0 input)
+
+
+
+#reset-options " --max_fuel 0 --z3rlimit 100"
+
 val uint64s_to_be_bytes:
   output:uint8_p ->
   input:buffer H64.t{disjoint output input} ->
